src/semantics.v
@@ -10,9 +10,7 @@ Import syntax.
 
 Section semantics.
 
-  Context {get_contract_type : contract_constant -> M type}.
-
-  Implicit Types (get_contract_type : contract_constant -> M type).
+  Context {get_contract_type : contract_constant -> M type} {parameter_ty : type}.
 
   Fixpoint data (a : type) {struct a} : Set :=
     match a with
@@ -29,7 +27,8 @@ Section semantics.
     | set_ a => set.set (comparable_data a) (compare a)
     | map a b => map.map (comparable_data a) (data b) (compare a)
     | big_map a b => map.map (comparable_data a) (data b) (compare a)
-    | lambda a b => @instruction get_contract_type (a ::: nil) (b ::: nil)
+    | lambda a b =>
+      @instruction get_contract_type parameter_ty (a ::: nil) (b ::: nil)
     | contract a => {s : contract_constant | get_contract_type s = Return _ a }
     end.
 
@@ -57,7 +56,7 @@ Section semantics.
         contract_ : forall p, data address -> M (option (data (contract p)));
         source : M (data address);
         sender : M (data address);
-        self : forall p, M (data (contract p));
+        self : data (contract parameter_ty);
         amount : M tez.mutez;
         implicit_account :
           comparable_data key_hash -> M (data (contract unit));
@@ -95,7 +94,7 @@ Section semantics.
     | Key_constant x => Mk_key x
     | Key_hash_constant x => Mk_key_hash x
     | Mutez_constant (Mk_mutez x) => x
-    | @Contract_constant _ a x H => exist _ x H
+    | @Contract_constant _ _ a x H => exist _ x H
     | Unit => tt
     | True_ => true
     | False_ => false
@@ -105,7 +104,7 @@ Section semantics.
     | Some_ a => Some (concrete_data_to_data _ a)
     | None_ => None
     | Concrete_list l => List.map (concrete_data_to_data _) l
-    | @Concrete_set _ a l =>
+    | @Concrete_set _ _ a l =>
       (fix concrete_data_set_to_data (l : list (concrete_data a)) :=
          match l with
          | nil => set.empty _ _
@@ -119,7 +118,7 @@ Section semantics.
              (concrete_data_to_data a x)
              (concrete_data_set_to_data l)
          end) l
-    | @Concrete_map _ a b l =>
+    | @Concrete_map _ _ a b l =>
       (fix concrete_data_map_to_data
            (l : Datatypes.list (elt_pair (concrete_data a) (concrete_data b))) :=
          match l with
@@ -345,7 +344,7 @@ Section semantics.
     | O => fun SA => Failed _ Out_of_fuel
     | S n =>
       match i in instruction A B return stack A -> M (stack B) with
-      | @FAILWITH _ A B a =>
+      | @FAILWITH _ _ A B a =>
         fun '(x, _) => Failed _ (Assertion_Failure (data a) x)
 
       (* According to the documentation, FAILWITH's argument should
@@ -383,53 +382,53 @@ Section semantics.
       | GT => fun '(x, SA) => Return _ ((x >? 0)%Z, SA)
       | LE => fun '(x, SA) => Return _ ((x <=? 0)%Z, SA)
       | GE => fun '(x, SA) => Return _ ((x >=? 0)%Z, SA)
-      | @OR _ _ s =>
+      | @OR _ _ _ s =>
         fun '(x, (y, SA)) => Return _ (or_fun _ (bitwise_variant_field _ s) x y, SA)
-      | @AND _ _ s =>
+      | @AND _ _ _ s =>
         fun '(x, (y, SA)) => Return _ (and _ (bitwise_variant_field _ s) x y, SA)
-      | @XOR _ _ s =>
+      | @XOR _ _ _ s =>
         fun '(x, (y, SA)) => Return _ (xor _ (bitwise_variant_field _ s) x y, SA)
-      | @NOT _ _ s =>
+      | @NOT _ _ _ s =>
         fun '(x, SA) => Return _ (not _ _ (not_variant_field _ s) x, SA)
-      | @NEG _ _ s =>
+      | @NEG _ _ _ s =>
         fun '(x, SA) => Return _ (neg _ (neg_variant_field _ s) x, SA)
       | ABS => fun '(x, SA) => Return _ (Z.abs_N x, SA)
-      | @ADD _ _ _ s =>
+      | @ADD _ _ _ _ s =>
         fun '(x, (y, SA)) =>
           bind (fun r => Return _ (r, SA))
                (add _ _ _ (add_variant_field _ _ s) x y)
-      | @SUB _ _ _ s =>
+      | @SUB _ _ _ _ s =>
         fun '(x, (y, SA)) =>
           bind (fun r => Return _ (r, SA))
                (sub _ _ _ (sub_variant_field _ _ s) x y)
-      | @MUL _ _ _ s =>
+      | @MUL _ _ _ _ s =>
         fun '(x, (y, SA)) =>
           bind (fun r => Return _ (r, SA))
                (mul _ _ _ (mul_variant_field _ _ s) x y)
-      | @EDIV _ _ _ s =>
+      | @EDIV _ _ _ _ s =>
         fun '(x, (y, SA)) =>
           Return _ (ediv _ _ _ _ (ediv_variant_field _ _ s) x y, SA)
       | LSL => fun '(x, (y, SA)) => Return _ (N.shiftl x y, SA)
       | LSR => fun '(x, (y, SA)) => Return _ (N.shiftr x y, SA)
       | COMPARE =>
         fun '(x, (y, SA)) => Return _ (comparison_to_int (compare _ x y), SA)
-      | @CONCAT _ _ s =>
+      | @CONCAT _ _ _ s =>
         fun '(x, (y, SA)) =>
           Return _ (concat _ (stringlike_variant_field _ s) x y, SA)
-      | @SLICE _ _ i =>
+      | @SLICE _ _ _ i =>
         fun '(n1, (n2, (s, SA))) =>
           Return _ (slice _ (stringlike_variant_field _ i) n1 n2 s, SA)
       | PAIR => fun '(x, (y, SA)) => Return _ ((x, y), SA)
       | CAR => fun '((x, y), SA) => Return _ (x, SA)
       | CDR => fun '((x, y), SA) => Return _ (y, SA)
       | EMPTY_SET a => fun SA => Return _ (set.empty _ (compare a), SA)
-      | @MEM _ _ _ s =>
+      | @MEM _ _ _ _ s =>
         fun '(x, (y, SA)) =>
           Return _ (mem _ _ (mem_variant_field _ _ s) x y, SA)
-      | @UPDATE _ _ _ _ s =>
+      | @UPDATE _ _ _ _ _ s =>
         fun '(x, (y, (z, SA))) =>
           Return _ (update _ _ _ (update_variant_field _ _ _ s) x y z, SA)
-      | @ITER _ _ s _ body =>
+      | @ITER _ _ _ s _ body =>
         fun '(x, SA) =>
           match iter_destruct _ _ (iter_variant_field _ s) x with
           | None => Return _ SA
@@ -438,14 +437,14 @@ Section semantics.
                     eval (ITER body) n (y, SB))
                  (eval body n (a, SA))
           end
-      | @SIZE _ _ s =>
+      | @SIZE _ _ _ s =>
         fun '(x, SA) => Return _ (N.of_nat (size _ (size_variant_field _ s) x), SA)
       | EMPTY_MAP k val =>
         fun SA => Return _ (map.empty (comparable_data k) (data val) _, SA)
-      | @GET _ _ _ s =>
+      | @GET _ _ _ _ s =>
         fun '(x, (y, SA)) =>
           Return _ (get _ _ _ (get_variant_field _ _ s) x y, SA)
-      | @MAP _ _ _ s _ body =>
+      | @MAP _ _ _ _ s _ body =>
         let v := (map_variant_field _ _ s) in
         fun '(x, SA) =>
           match map_destruct _ _ _ _ v x with
@@ -515,7 +514,7 @@ Section semantics.
         fun '(x, SA) => bind (fun r => Return _ (r, SA)) (contract_ nd _ x)
       | SOURCE => fun SA => bind (fun r => Return _ (r, SA)) (source nd)
       | SENDER => fun SA => bind (fun r => Return _ (r, SA)) (sender nd)
-      | SELF => fun SA => bind (fun r => Return _ (r, SA)) (self nd _)
+      | SELF => fun SA => Return _ (self nd, SA)
       | AMOUNT => fun SA => bind (fun r => Return _ (r, SA)) (amount nd)
       | IMPLICIT_ACCOUNT =>
         fun '(x, SA) => bind (fun r => Return _ (r, SA)) (implicit_account nd x)
@@ -695,50 +694,50 @@ Section semantics.
     | GT => fun psi '(x, SA) => psi ((x >? 0)%Z, SA)
     | LE => fun psi '(x, SA) => psi ((x <=? 0)%Z, SA)
     | GE => fun psi '(x, SA) => psi ((x >=? 0)%Z, SA)
-    | @OR _ _ s =>
+    | @OR _ _ _ s =>
       fun psi '(x, (y, SA)) => psi (or_fun _ (bitwise_variant_field _ s) x y, SA)
-    | @AND _ _ s =>
+    | @AND _ _ _ s =>
       fun psi '(x, (y, SA)) => psi (and _ (bitwise_variant_field _ s) x y, SA)
-    | @XOR _ _ s =>
+    | @XOR _ _ _ s =>
       fun psi '(x, (y, SA)) => psi (xor _ (bitwise_variant_field _ s) x y, SA)
-    | @NOT _ _ s =>
+    | @NOT _ _ _ s =>
       fun psi '(x, SA) => psi (not _ _ (not_variant_field _ s) x, SA)
-    | @NEG _ _ s =>
+    | @NEG _ _ _ s =>
       fun psi '(x, SA) => psi (neg _ (neg_variant_field _ s) x, SA)
     | ABS => fun psi '(x, SA) => psi (Z.abs_N x, SA)
-    | @ADD _ _ _ s =>
+    | @ADD _ _ _ _ s =>
       fun psi '(x, (y, SA)) =>
         precond (add _ _ _ (add_variant_field _ _ s) x y) (fun z => psi (z, SA))
-    | @SUB _ _ _ s =>
+    | @SUB _ _ _ _ s =>
       fun psi '(x, (y, SA)) =>
         precond (sub _ _ _ (sub_variant_field _ _ s) x y) (fun z => psi (z, SA))
-    | @MUL _ _ _ s =>
+    | @MUL _ _ _ _ s =>
       fun psi '(x, (y, SA)) =>
         precond (mul _ _ _ (mul_variant_field _ _ s) x y) (fun z => psi (z, SA))
-    | @EDIV _ _ _ s =>
+    | @EDIV _ _ _ _ s =>
       fun psi '(x, (y, SA)) =>
         psi (ediv _ _ _ _ (ediv_variant_field _ _ s) x y, SA)
     | LSL => fun psi '(x, (y, SA)) => psi (N.shiftl x y, SA)
     | LSR => fun psi '(x, (y, SA)) => psi (N.shiftr x y, SA)
     | COMPARE =>
       fun psi '(x, (y, SA)) => psi (comparison_to_int (compare _ x y), SA)
-    | @CONCAT _ _ s =>
+    | @CONCAT _ _ _ s =>
       fun psi '(x, (y, SA)) =>
         psi (concat _ (stringlike_variant_field _ s) x y, SA)
-    | @SLICE _ _ i =>
+    | @SLICE _ _ _ i =>
       fun psi '(n1, (n2, (s, SA))) =>
         psi (slice _ (stringlike_variant_field _ i) n1 n2 s, SA)
     | PAIR => fun psi '(x, (y, SA)) => psi ((x, y), SA)
     | CAR => fun psi '((x, y), SA) => psi (x, SA)
     | CDR => fun psi '((x, y), SA) => psi (y, SA)
     | EMPTY_SET a => fun psi SA => psi (set.empty _ (compare a), SA)
-    | @MEM _ _ _ s =>
+    | @MEM _ _ _ _ s =>
       fun psi '(x, (y, SA)) =>
         psi (mem _ _ (mem_variant_field _ _ s) x y, SA)
-    | @UPDATE _ _ _ _ s =>
+    | @UPDATE _ _ _ _ _ s =>
       fun psi '(x, (y, (z, SA))) =>
         psi (update _ _ _ (update_variant_field _ _ _ s) x y z, SA)
-    | @ITER _ _ s _ body =>
+    | @ITER _ _ _ s _ body =>
       fun psi '(x, SA) =>
         match iter_destruct _ _ (iter_variant_field _ s) x with
         | None => psi SA
@@ -747,13 +746,13 @@ Section semantics.
                        (fun SB => eval_precond_n (ITER body) psi (y, SB))
                        (a, SA)
         end
-    | @SIZE _ _ s =>
+    | @SIZE _ _ _ s =>
       fun psi '(x, SA) => psi (N.of_nat (size _ (size_variant_field _ s) x), SA)
     | EMPTY_MAP k val =>
       fun psi SA => psi (map.empty (comparable_data k) (data val) _, SA)
-    | @GET _ _ _ s =>
+    | @GET _ _ _ _ s =>
       fun psi '(x, (y, SA)) => psi (get _ _ _ (get_variant_field _ _ s) x y, SA)
-    | @MAP _ _ _ s _ body =>
+    | @MAP _ _ _ _ s _ body =>
       let v := (map_variant_field _ _ s) in
       fun psi '(x, SA) =>
         match map_destruct _ _ _ _ v x with
@@ -823,7 +822,7 @@ Section semantics.
       fun psi '(x, SA) => precond_ex (contract_ nd _ x) (fun r => psi (r, SA))
     | SOURCE => fun psi SA => precond_ex (source nd) (fun r => psi (r, SA))
     | SENDER => fun psi SA => precond_ex (sender nd) (fun r => psi (r, SA))
-    | SELF => fun psi SA => precond_ex (self nd _) (fun r => psi (r, SA))
+    | SELF => fun psi SA => psi (self nd, SA)
     | AMOUNT => fun psi SA => precond_ex (amount nd) (fun r => psi (r, SA))
     | IMPLICIT_ACCOUNT =>
       fun psi '(x, SA) => precond_ex (implicit_account nd x) (fun r => psi (r, SA))
@@ -1003,10 +1002,7 @@ Section semantics.
       rewrite <- precond_exists.
       apply precond_eqv.
       reflexivity.
-    - rewrite precond_bind.
-      rewrite <- precond_exists.
-      apply precond_eqv.
-      reflexivity.
+    - reflexivity.
     - rewrite precond_bind.
       rewrite <- precond_exists.
       apply precond_eqv.
